src/Spec/WeakestPreconditions.v
@@ -14,122 +14,74 @@ Section Dynamics.
 
   Definition precondition T := forall (post: T -> State -> Prop), State -> Prop.
 
-  Context (op_wp: forall T, Op T -> precondition T).
-
-  Definition op_wp_ok :=
-    forall T (op:Op T) post s, op_wp op post s ->
-                          forall s' v, step op s s' v ->
-                                  post v s'.
-
-  Fixpoint wp T (p: proc T)
-    : precondition T :=
-    fun post =>
-      match p with
-      | Ret v => post v
-      | Prim op => op_wp op post
-      | Bind p rx =>
-        wp p (fun v s' => wp (rx v) post s')
-      end.
+  Record WPSetup :=
+    { op_wp: forall T, Op T -> precondition T;
+      op_wp_ok :
+        forall T (op:Op T) post s, op_wp op post s ->
+                              forall s' v, step op s s' v ->
+                                      post v s'; }.
 
   Ltac cleanup :=
     simpl in *;
     unfold pure, and_then, test, rel_or in *;
     propositional.
 
+  Context (wp: WPSetup).
+
+  Fixpoint precond T (p: proc T)
+    : precondition T :=
+    fun post =>
+      match p with
+      | Ret v => post v
+      | Prim op => wp.(op_wp) op post
+      | Bind p rx =>
+        precond p (fun v s' => precond (rx v) post s')
+      end.
+
   Theorem wp_ok :
-    op_wp_ok ->
     forall T (p: proc T) (post: T -> State -> Prop),
-    forall s, wp p post s ->
+    forall s, precond p post s ->
          forall s' v, exec p s s' v ->
                  post v s'.
   Proof.
     intros Hop_wp.
     induction p; cleanup; eauto.
-    - eapply Hop_wp in H; eauto.
+    - eapply wp.(op_wp_ok) in H; eauto.
     - eapply IHp in H1; eauto; cleanup.
       eapply H in H1; eauto.
   Qed.
 
-  Theorem wp_op_kat :
-    (forall T (op:Op T) post,
-        test (op_wp op post);; step op --->
-             test (op_wp op post);; v <- step op; test (post v);; pure v) ->
-    op_wp_ok.
-  Proof.
-    unfold op_wp_ok.
-    cleanup.
-    specialize (H _ op post s s' v); simpl in H.
-    match type of H with
-    | ?P -> _ =>
-      let HP := fresh in
-      assert P as HP; [ | specialize (H HP); propositional ]
-    end.
-    descend; intuition eauto.
-  Qed.
-
-  Theorem wp_kat
-          T (p: proc T) (post: T -> State -> Prop) :
-    (forall T (op:Op T) post,
-        test (op_wp op post);; step op --->
-             test (op_wp op post);; v <- step op; test (post v);; pure v) ->
-    test (wp p post);; exec p --->
-         test (wp p post);; v <- exec p; test (post v);; pure v.
-  Proof.
-    cleanup; unfold rimpl; propositional.
-    descend; intuition eauto.
-    descend; intuition eauto.
-    descend; intuition eauto.
-    eapply wp_ok; eauto.
-    eapply wp_op_kat; eauto.
-  Qed.
-
   Definition crashpre := forall (crash: State -> Prop), State -> Prop.
 
-  Fixpoint wp_crash T (p: proc T) : crashpre :=
+  Fixpoint crashcond T (p: proc T) : crashpre :=
     fun crash s =>
       match p with
       | Ret v => crash s
       | Prim op => crash s /\
-                  op_wp op (fun v s => crash s) s
+                  wp.(op_wp) op (fun v s => crash s) s
       | Bind p rx =>
         (* crashing at s is handled by wp_crash p (inductively; the other two
  rules includes this *)
-        wp_crash p crash s /\
-        wp p (fun v s' => wp_crash (rx v) crash s') s
+        crashcond p crash s /\
+        precond p (fun v s' => crashcond (rx v) crash s') s
       end.
 
   Theorem wp_crash_ok T (p: proc T) (crash: State -> Prop) :
-    op_wp_ok ->
-    forall s, wp_crash p crash s ->
+    forall s, crashcond p crash s ->
          forall s' v, exec_crash p s s' v ->
                  crash s'.
   Proof.
-    intros Hop_ok.
     induction p; cleanup; eauto.
     - repeat match goal with
              | [ H: _ \/ _ |- _ ] => destruct H; propositional; eauto
              end.
-      eapply Hop_ok in H1; eauto; cleanup.
+      eapply wp.(op_wp_ok) in H1; eauto; cleanup.
     - repeat match goal with
              | [ H: _ \/ _ |- _ ] => destruct H; propositional; eauto
              end.
       + eapply IHp; eauto.
         apply exec_crash_noop; cleanup; eauto.
       + eapply wp_ok in H2; eauto.
-  Qed.
-
-  Theorem wp_crash_kat T (p: proc T) (crash: State -> Prop) :
-    (forall T (op:Op T) post,
-        test (op_wp op post);; step op --->
-             test (op_wp op post);; v <- step op; test (post v);; pure v) ->
-    test (wp_crash p crash);; exec_crash p --->
-         test (wp_crash p crash);; exec_crash p;; test crash.
-  Proof.
-    cleanup; unfold rimpl; propositional.
-    descend; intuition eauto.
-    descend; intuition eauto.
-    eapply wp_crash_ok; eauto.
-    eapply wp_op_kat; eauto.
   Qed.
 
 End Dynamics.
