src/Spec/WpRefine.v
@@ -1,0 +1,30 @@
+From Tactical Require Import Propositional.
+
+Require Import Helpers.RelationAlgebra.
+
+Require Import Spec.Proc.
+Require Import Spec.WeakestPreconditions.
+Require Import Spec.Abstraction.
+
+Section Dynamics.
+  Context `(sem: Dynamics Op State).
+  Notation proc := (proc Op).
+  Notation step := sem.(step).
+  Notation exec := sem.(exec).
+
+  Context AState (absr: relation AState State unit).
+  Context (wp: WPSetup sem).
+
+  Theorem wp_refine T (p: proc T) (r: relation AState AState T) :
+    (forall s s__a, absr s__a s tt ->
+             wp.(precond) p (fun v s' =>
+                               exists s__a', r s__a s__a' v /\
+                                      absr s__a' s' tt) s) ->
+    refines absr (exec p) r.
+  Proof.
+    intros.
+    eapply refine_unfolded; intros.
+    eapply H in H0; eauto.
+    eapply wp_ok in H0; eauto.
+  Qed.
+End Dynamics.
